\documentclass[UTF8,a4paper,10pt]{article}

% \begin{equation**}
%   \begin{aligned}
%   \end{aligned}
% \end{equation*}

% \begin{mybox}{}
% \end{mybox}


% \begin{Problem}[]{}
% \end{Problem}

% \begin{solution}\,
% \end{solution}
  

% \begin{enumerate}[label=(\alph*)]
% \end{enumerate} 

% \setcounter{section}{3} 
% \setcounter{theorem}{3}

% \begin{theorem}\label{thm:3.4}
%   If $E = \bigsqcup_{k} E_k$ is a countable union of sets, then $|E|_e \leq \sum_{k} |E_k|_e$.
%   \end{theorem}

%  \footcite[][42]{Wheeden_Zygmund_2015}

\input{preamble.tex}

\begin{document}




\begin{Problem}[]{The Prékopa-Leindler Inequality}
  Let $0 < \lambda < 1$ and let $f$, $g$ and $h$ be non-negative integrable functions on $\mathbb{R}^n$ satisfying for every $x, y \in \mathbb{R}^n$, one has
  $$
  h\left((1 - \lambda)x + \lambda y\right) \geq f(x)^{1-\lambda} g(y)^\lambda.
  $$
  Show that
  $$
  \int_{\mathbb{R}^n} h(x) \, dx \geq \left(\int_{\mathbb{R}^n} f(x) \, dx\right)^{1-\lambda} \left(\int_{\mathbb{R}^n} g(x) \, dx\right)^\lambda.
  $$
  
\end{Problem}

First, consider the case \(n=1\).


Without loss of generality, we may assume that
\begin{equation}
\int_{\mathbb{R}} f(x) \, dx = F > 0 \quad \text{and} \quad \int_{\mathbb{R}} g(x) \, dx = G > 0.
\end{equation}
Define $u, v : (0, 1) \rightarrow \mathbb{R}$ such that $u(t)$ and $v(t)$ are the smallest numbers satisfying
\begin{equation}\label{eq.28}
\frac{1}{F} \int_{-\infty}^{u(t)} f(x) \, dx = \frac{1}{G} \int_{-\infty}^{v(t)} g(x) \, dx = t.
\end{equation}
Then $u$ and $v$ may be discontinuous, but they are strictly increasing functions and so are differentiable almost everywhere. Let
\begin{equation}
w(t) = (1 - \lambda)u(t) + \lambda v(t).
\end{equation}
Take the derivative of \eqref{eq.28} with respect to $t$ to obtain
\begin{equation}
\frac{f(u(t)) u'(t)}{F} = \frac{g(v(t)) v'(t)}{G} = 1.
\end{equation}

Using this and the arithmetic-geometric mean inequality, we obtain (when $f'(u(t)) \neq 0$ and $g'(v(t)) \neq 0$)


\begin{equation}
\begin{aligned}
w'(t) = (1 - \lambda)u'(t) + \lambda v'(t) &\geq \left(\frac{u'(t)}{1-\lambda}\right)^{1-\lambda} \left(\frac{v'(t)}{\lambda}\right)^\lambda\\
 &= \left(\frac{F}{f'(u(t))}\right)^{1-\lambda} \left(\frac{G}{g'(v(t))}\right)^\lambda.
\end{aligned}
\end{equation}

Therefore

\begin{equation}
  \begin{aligned}
\int_{\mathbb{R}} h(x) \, dx &= \int_{0}^{1} h(w(t)) w'(t) \, dt \\
&\geq \int_{0}^{1} \left(f'(u(t))\right)^{1-\lambda} \left(g'(v(t))\right)^\lambda \left(\frac{F}{f'(u(t))}\right)^{1-\lambda} \left(\frac{G}{g'(v(t))}\right)^\lambda \, dt \\
&= F^{1-\lambda}G^\lambda.
\end{aligned}
\end{equation}  



Next, we perform the induction on $n$. 

Let's indicate the variables as $x = (x_1, x') \in \mathbb{R} \times \mathbb{R}^{n-1}$ and define the functions
\begin{align*}
F(x_1) &= \int_{\mathbb{R}^{n-1}} f(x_1, x') \, dx', \\
G(y_1) &= \int_{\mathbb{R}^{n-1}} g(y_1, y') \, dy', 
\\
H(z_1) &= \int_{\mathbb{R}^{n-1}} f(z_1, z') \, dz'
.
\end{align*}
Fix $x_1, y_1, z_1 \in \mathbb{R}$ such that $z_1 = (1 - \lambda)x_1 + \lambda y_1$. Then
\[
h(z_1, z') \geq f(x_1, x')^{1-\lambda} g(y_1, y')^\lambda
\]
for all $x', y', z' \in \mathbb{R}^{n-1}$ with $z' = (1-\lambda)x' + \lambda y'$. By induction, Prékopa-Leindler holds in dimension $n - 1$, thus it follows that
\[
H(z_1) \geq F(x_1)^{1-\lambda} G(y_1)^\lambda.
\]
So now we can apply again the 1-dimensional Prékopa-Leindler inequality to obtain the desired conclusion.



\pagebreak
\begin{Problem}[]{The Brunn-Minkowski Inequality}

  Let $0 < \lambda < 1$ and let $A$ and $B$ be non-empty bounded measurable sets in $\mathbb{R}^n$ such that ${(1 - \lambda)A + \lambda B}$ is also measurable. Show that
$$
|A + B|^\frac{1}{n} \geq |A|^\frac{1}{n} + |B|^\frac{1}{n}.
$$

\end{Problem}

Let

\begin{equation*}
  \begin{aligned}
    f(x) &= \Id_{A},\\
    g(x) &= \Id_{B},\\
    h(x) &= \Id_{(1-\lambda)A+\lambda B}.
\end{aligned}
\end{equation*}  

Applying the Prékopa-Leindler Inequality, we have that 
\begin{equation*}
  |(1-\lambda)A+\lambda B| \geq {|A|}^{1-\lambda} |B|^{\lambda}.
\end{equation*}

Now show that this inequality (multiplicative BM) implies the additive version\(|A + B|^\frac{1}{n} \geq |A|^\frac{1}{n} + |B|^\frac{1}{n}\):

We assume that both \(A, B\) have positive volume, as otherwise the inequality is trivial, and normalize them to have volume 1 by setting
\[
A' = \frac{A}{|A|^{1/n}}, \quad B' = \frac{B}{|B|^{1/n}}.
\]
We define \(\lambda'\) by
\[
\lambda'  = \frac{\lambda |B|^{1/n}}{(1-\lambda)|A|^{1/n} + \lambda |B|^{1/n}}, \quad 1 - \lambda' = \frac{(1-\lambda)|A|^{1/n}}{(1-\lambda)|A|^{1/n} + \lambda |B|^{1/n}}.
\]
With these definitions, and using that \(|A'| = |B'| = 1\), we calculate using the multiplicative Brunn--Minkowski inequality that:
\[
\left| \frac{(1 - \lambda) A + \lambda B}{(1 - \lambda)|A|^{1/n} + \lambda |B|^{1/n}} \right| = \left| (1 - \lambda') A' + \lambda' B' \right| \geq |A'|^{1-\lambda'} |B'|^{\lambda'} = 1.
\]
The additive form of Brunn--Minkowski now follows by pulling the scaling out of the leftmost volume calculation and rearranging:

\[
\left| (1 - \lambda) A + \lambda B\right| \geq  \left\{(1 - \lambda)|A|^{1/n} + \lambda |B|^{1/n}\right\}^n.
\]

\[
{\left| (1 - \lambda) A + \lambda B \right|}^{1/n} \geq (1 - \lambda)|A|^{1/n} + \lambda |B|^{1/n}
\]

Set \(\lambda = 1/2\), 

\begin{equation*}
  \begin{aligned}
    {\left| \frac{1}{2} A +  \frac{1}{2} B \right|}^{1/n}  
    &= \frac{1}{2} {\left|  A + B \right|}^{1/n} 
    \\
    &\geq \frac{1}{2}|A|^{1/n} + \frac{1}{2} |B|^{1/n}
  \end{aligned}
\end{equation*}
\(\implies\)
$$
|A + B|^\frac{1}{n} \geq |A|^\frac{1}{n} + |B|^\frac{1}{n}.
$$

\end{document}